
\documentclass[12pt]{article}
%%%%%%%%%%%%%%%%%%%%%%%%%%%%%%%%%%%%%%%%%%%%%%%%%%%%%%%%%%%%%%%%%%%%%%%%%%%%%%%%%%%%%%%%%%%%%%%%%%%%%%%%%%%%%%%%%%%%%%%%%%%%%%%%%%%%%%%%%%%%%%%%%%%%%%%%%%%%%%%%%%%%%%%%%%%%%%%%%%%%%%%%%%%%%%%%%%%%%%%%%%%%%%%%%%%%%%%%%%%%%%%%%%%%%%%%%%%%%%%%%%%%%%%%%%%%
%TCIDATA{OutputFilter=LATEX.DLL}
%TCIDATA{Version=5.50.0.2953}
%TCIDATA{<META NAME="SaveForMode" CONTENT="1">}
%TCIDATA{BibliographyScheme=Manual}
%TCIDATA{Created=Wednesday, May 17, 2006 13:09:49}
%TCIDATA{LastRevised=Thursday, March 05, 2009 15:00:11}
%TCIDATA{<META NAME="GraphicsSave" CONTENT="32">}
%TCIDATA{<META NAME="DocumentShell" CONTENT="Standard LaTeX\Blank - Standard LaTeX Article">}
%TCIDATA{CSTFile=40 LaTeX article.cst}

\newtheorem{theorem}{Theorem}
\newtheorem{acknowledgement}[theorem]{Acknowledgement}
\newtheorem{algorithm}[theorem]{Algorithm}
\newtheorem{axiom}[theorem]{Axiom}
\newtheorem{case}[theorem]{Case}
\newtheorem{claim}[theorem]{Claim}
\newtheorem{conclusion}[theorem]{Conclusion}
\newtheorem{condition}[theorem]{Condition}
\newtheorem{conjecture}[theorem]{Conjecture}
\newtheorem{corollary}[theorem]{Corollary}
\newtheorem{criterion}[theorem]{Criterion}
\newtheorem{definition}[theorem]{Definition}
\newtheorem{example}[theorem]{Example}
\newtheorem{exercise}[theorem]{Exercise}
\newtheorem{lemma}[theorem]{Lemma}
\newtheorem{notation}[theorem]{Notation}
\newtheorem{problem}[theorem]{Problem}
\newtheorem{proposition}[theorem]{Proposition}
\newtheorem{remark}[theorem]{Remark}
\newtheorem{solution}[theorem]{Solution}
\newtheorem{summary}[theorem]{Summary}
\newenvironment{proof}[1][Proof]{\noindent\textbf{#1.} }{\ \rule{0.5em}{0.5em}}
\input{tcilatex}
\begin{document}


\section{Model}

\[
y_{ig}=X_{i}\beta +\left( \bar{X}_{g}\beta \right) \gamma +\mu
_{g}+\varepsilon _{i}+\xi _{i}
\]%
\qquad 
\begin{eqnarray*}
\mu _{g} &\mid &\bar{X}_{g}\sim N\left( 0,\tau ^{2}\right)  \\
\varepsilon _{i} &\mid &\bar{X}_{g},X_{i},\mu _{g}\sim N\left( 0,\sigma
^{2}\right)  \\
\xi _{i} &\mid &\bar{X}_{g},X_{i},\mu _{g},\varepsilon _{i}\sim N\left(
0,r_{i}\right) .
\end{eqnarray*}%
Comments:

\begin{itemize}
\item $\mu _{g}$ is group random effect

\item $\gamma $ allows for group effects to be correlated with average group
characteristics

\item $\varepsilon _{i}$ is individual shock

\item $\xi _{i}$ is measurement error with known variance $r_{i}$ that can
vary by individual.
\end{itemize}

\section{Likelihood}

The likelihood function for group $g$ is%
\[
L_{g}=\int_{-\infty }^{\infty }\phi \left( \frac{\mu _{g}}{\tau }\right)
\prod_{i=1}^{T_{g}}\phi \left( \frac{y_{ig}-X_{i}\beta -\left( \bar{X}%
_{g}\beta \right) \gamma -\mu _{g}}{\sqrt{\sigma ^{2}+r_{i}}}\right) d\mu
_{g}
\]%
Let%
\[
\tilde{y}_{ig}=y_{ig}-X_{i}\beta -\left( \bar{X}_{g}\beta \right) \gamma 
\]%
and let%
\[
\tilde{\sigma}_{i}^{2}=\sigma ^{2}+r_{i}.
\]%
Then likelihood can be written as%
\[
\ln L_{g}=-\frac{1}{2}\left[ \sum_{i=1}^{T_{g}}\ln \left( \tilde{\sigma}%
_{i}^{2}\right) +\ln \left( 1+\tau ^{2}\sum_{i=1}^{T_{g}}\frac{1}{\tilde{%
\sigma}_{i}^{2}}\right) +\sum_{i=1}^{T_{g}}\frac{\tilde{y}_{ig}^{2}}{\tilde{%
\sigma}_{i}^{2}}-\left( \frac{1}{\tau ^{2}}+\sum_{i=1}^{T_{g}}\frac{1}{%
\tilde{\sigma}_{i}^{2}}\right) ^{-1}\left( \sum_{i=1}^{T_{g}}\frac{\tilde{y}%
_{ig}}{\tilde{\sigma}_{i}^{2}}\right) ^{2}\right] 
\]%
following derivation below.

Note that in the case that $\gamma =\eta =0$, the likelihood becomes%
\[
\ln L_{g}=-\frac{1}{2}\left\{ \frac{1}{\sigma ^{2}}\left[ \sum_{i=1}^{T_{g}}%
\left( y_{ig}-X_{i}\beta \right) ^{2}-\frac{\tau ^{2}}{T_{g}\tau ^{2}+\sigma
^{2}}\left( \sum_{i=1}^{T_{g}}\left( y_{ig}-X_{i}\beta \right) \right) ^{2}%
\right] +\ln \left( T_{g}\frac{\tau ^{2}}{\sigma ^{2}}+1\right) +T_{g}\ln
\left( \sigma ^{2}\right) \right\} 
\]%
Borrowing from the Stata manual, if we put the constant term back in\
(irrelevant for maximization \&\ derivatives) we have%
\[
\ln L_{g}=-\frac{1}{2}\left[ \sum_{i=1}^{T_{g}}\ln \left( \tilde{\sigma}%
_{i}^{2}\right) +\ln \left( 1+\tau ^{2}\sum_{i=1}^{T_{g}}\frac{1}{\tilde{%
\sigma}_{i}^{2}}\right) +\sum_{i=1}^{T_{g}}\frac{\tilde{y}_{ig}^{2}}{\tilde{%
\sigma}_{i}^{2}}-\left( \frac{1}{\tau ^{2}}+\sum_{i=1}^{T_{g}}\frac{1}{%
\tilde{\sigma}_{i}^{2}}\right) ^{-1}\left( \sum_{i=1}^{T_{g}}\frac{\tilde{y}%
_{ig}}{\tilde{\sigma}_{i}^{2}}\right) ^{2}+T_{g}\ln \left( 2\pi \right) %
\right] 
\]

\section{First Derivatives}

\begin{eqnarray*}
\frac{\partial \left( \ln L_{g}\right) }{\partial \beta } &=&%
\sum_{i=1}^{T_{g}}\frac{\partial \left( \ln L_{g}\right) }{\partial \left(
X_{i}\beta \right) }X_{i} \\
\frac{\partial \left( \ln L_{g}\right) }{\partial \left( X_{i}\beta \right) }
&=&\left( 1+\frac{\gamma }{T_{g}}\right) \left( \frac{\tilde{y}_{ig}}{\tilde{%
\sigma}_{i}^{2}}-\left( \sum_{i=1}^{T_{g}}\frac{\tilde{y}_{ig}}{\tilde{\sigma%
}_{i}^{2}}\right) \left( \frac{1}{\tilde{\sigma}_{i}^{2}}\right) \left( 
\frac{1}{\tau ^{2}}+\sum_{i=1}^{T_{g}}\frac{1}{\tilde{\sigma}_{i}^{2}}%
\right) ^{-1}\right)
\end{eqnarray*}%
\[
\frac{\partial \left( \ln L_{g}\right) }{\partial \sigma }=-\sigma \left[
\sum_{i=1}^{T_{g}}\frac{1}{\tilde{\sigma}_{i}^{2}}-\frac{\tau ^{2}\left(
\sum_{i=1}^{T_{g}}\frac{1}{\tilde{\sigma}_{i}^{4}}\right) }{1+\tau
^{2}\left( \sum_{i=1}^{T_{g}}\frac{1}{\tilde{\sigma}_{i}^{2}}\right) }%
-\sum_{i=1}^{T_{g}}\frac{\tilde{y}_{ig}^{2}}{\tilde{\sigma}_{i}^{4}}+2\left(
\sum_{i=1}^{T_{g}}\frac{\tilde{y}_{ig}}{\tilde{\sigma}_{i}^{2}}\right)
\left( \sum_{i=1}^{T_{g}}\frac{\tilde{y}_{ig}}{\tilde{\sigma}_{i}^{4}}%
\right) \left( \frac{1}{\tau ^{2}}+\sum_{i=1}^{T_{g}}\frac{1}{\tilde{\sigma}%
_{i}^{2}}\right) ^{-1}-\left( \sum_{i=1}^{T_{g}}\frac{\tilde{y}_{ig}}{\tilde{%
\sigma}_{i}^{2}}\right) ^{2}\left( \sum_{i=1}^{T_{g}}\frac{1}{\tilde{\sigma}%
_{i}^{4}}\right) \left( \frac{1}{\tau ^{2}}+\sum_{i=1}^{T_{g}}\frac{1}{%
\tilde{\sigma}_{i}^{2}}\right) ^{-2}\right] 
\]%
\[
\frac{\partial \left( \ln L_{g}\right) }{\partial \tau }=-\tau \frac{%
\sum_{i=1}^{T_{g}}\frac{1}{\tilde{\sigma}_{i}^{2}}}{\left( 1+\tau
^{2}\sum_{i=1}^{T_{g}}\frac{1}{\tilde{\sigma}_{i}^{2}}\right) }+\frac{1}{%
\tau ^{3}}\left( \frac{1}{\tau ^{2}}+\sum_{i=1}^{T_{g}}\frac{1}{\tilde{\sigma%
}_{i}^{2}}\right) ^{-2}\left( \sum_{i=1}^{T_{g}}\frac{\tilde{y}_{ig}}{\tilde{%
\sigma}_{i}^{2}}\right) ^{2} 
\]%
\[
\frac{\partial \left( \ln L_{g}\right) }{\partial \gamma }=\left( \bar{X}%
_{g}\beta \right) \left( \sum_{i=1}^{T_{g}}\frac{\tilde{y}_{ig}}{\tilde{%
\sigma}_{i}^{2}}\right) \left[ 1-\left( \sum_{i=1}^{T_{g}}\frac{1}{\tilde{%
\sigma}_{i}^{2}}\right) \left( \frac{1}{\tau ^{2}}+\sum_{i=1}^{T_{g}}\frac{1%
}{\tilde{\sigma}_{i}^{2}}\right) ^{-1}\right] 
\]

\section{Derivation of Likelihood}

Substituting expression for normal pdf gives:%
\[
L_{g}=\frac{1}{2\pi }\frac{1}{\sqrt{\tau ^{2}}}\prod_{i=1}^{T_{g}}\frac{1}{%
\sqrt{\tilde{\sigma}_{i}^{2}}}\int_{-\infty }^{\infty }\exp \left( -\frac{1}{%
2}\frac{\mu _{g}^{2}}{\tau ^{2}}\right) \prod_{i=1}^{T_{g}}\exp \left( -%
\frac{1}{2}\frac{\left( \tilde{y}_{ig}-\mu _{g}\right) ^{2}}{\tilde{\sigma}%
_{i}^{2}}\right) d\mu _{g} 
\]%
Rewriting:%
\begin{eqnarray*}
L_{g} &=&\frac{1}{2\pi }\frac{1}{\sqrt{\tau ^{2}}}\prod_{i=1}^{T_{g}}\frac{1%
}{\sqrt{\tilde{\sigma}_{i}^{2}}}\int_{-\infty }^{\infty }\exp \left( -\frac{1%
}{2}\left( \frac{\mu _{g}^{2}}{\tau ^{2}}+\sum_{i=1}^{T_{g}}\frac{\left( 
\tilde{y}_{ig}-\mu _{g}\right) ^{2}}{\tilde{\sigma}_{i}^{2}}\right) \right)
d\mu _{g} \\
&=&\frac{1}{2\pi }\frac{1}{\sqrt{\tau ^{2}}}\prod_{i=1}^{T_{g}}\frac{1}{%
\sqrt{\tilde{\sigma}_{i}^{2}}}\int_{-\infty }^{\infty }\exp \left( -\frac{1}{%
2}\left( \frac{\mu _{g}^{2}}{\tau ^{2}}+\sum_{i=1}^{T_{g}}\frac{\tilde{y}%
_{ig}^{2}-2\tilde{y}_{ig}\mu _{g}+\mu _{g}^{2}}{\tilde{\sigma}_{i}^{2}}%
\right) \right) d\mu _{g} \\
&=&\frac{1}{2\pi }\frac{1}{\sqrt{\tau ^{2}}}\prod_{i=1}^{T_{g}}\frac{1}{%
\sqrt{\tilde{\sigma}_{i}^{2}}}\int_{-\infty }^{\infty }\exp \left( -\frac{1}{%
2}\left( \frac{\mu _{g}^{2}}{\tau ^{2}}+\sum_{i=1}^{T_{g}}\frac{1}{\tilde{%
\sigma}_{i}^{2}}\mu _{g}^{2}-2\mu _{g}\sum_{i=1}^{T_{g}}\frac{\tilde{y}_{ig}%
}{\tilde{\sigma}_{i}^{2}}+\sum_{i=1}^{T_{g}}\frac{\tilde{y}_{ig}^{2}}{\tilde{%
\sigma}_{i}^{2}}\right) \right) d\mu _{g} \\
&=&\frac{1}{2\pi }\frac{1}{\sqrt{\tau ^{2}}}\prod_{i=1}^{T_{g}}\frac{1}{%
\sqrt{\tilde{\sigma}_{i}^{2}}}\int_{-\infty }^{\infty }\exp \left( -\frac{1}{%
2}\left( \frac{1}{\tau ^{2}}+\sum_{i=1}^{T_{g}}\frac{1}{\tilde{\sigma}%
_{i}^{2}}\right) \left( \mu _{g}^{2}-2\mu _{g}\frac{\sum_{i=1}^{T_{g}}\frac{%
\tilde{y}_{ig}}{\tilde{\sigma}_{i}^{2}}}{\frac{1}{\tau ^{2}}%
+\sum_{i=1}^{T_{g}}\frac{1}{\tilde{\sigma}_{i}^{2}}}+\frac{\sum_{i=1}^{T_{g}}%
\frac{\tilde{y}_{ig}^{2}}{\tilde{\sigma}_{i}^{2}}}{\frac{1}{\tau ^{2}}%
+\sum_{i=1}^{T_{g}}\frac{1}{\tilde{\sigma}_{i}^{2}}}\right) \right) d\mu _{g}
\end{eqnarray*}%
Completing the square:%
\begin{eqnarray*}
L_{g} &=&\frac{1}{2\pi }\frac{1}{\sqrt{\tau ^{2}}}\prod_{i=1}^{T_{g}}\frac{1%
}{\sqrt{\tilde{\sigma}_{i}^{2}}}\int_{-\infty }^{\infty }\exp \left( -\frac{1%
}{2}\left( \frac{1}{\tau ^{2}}+\sum_{i=1}^{T_{g}}\frac{1}{\tilde{\sigma}%
_{i}^{2}}\right) \left( \mu _{g}^{2}-2\mu _{g}\frac{\sum_{i=1}^{T_{g}}\frac{%
\tilde{y}_{ig}}{\tilde{\sigma}_{i}^{2}}}{\frac{1}{\tau ^{2}}%
+\sum_{i=1}^{T_{g}}\frac{1}{\tilde{\sigma}_{i}^{2}}}+\left( \frac{%
\sum_{i=1}^{T_{g}}\frac{\tilde{y}_{ig}}{\tilde{\sigma}_{i}^{2}}}{\frac{1}{%
\tau ^{2}}+\sum_{i=1}^{T_{g}}\frac{1}{\tilde{\sigma}_{i}^{2}}}\right)
^{2}-\left( \frac{\sum_{i=1}^{T_{g}}\frac{\tilde{y}_{ig}}{\tilde{\sigma}%
_{i}^{2}}}{\frac{1}{\tau ^{2}}+\sum_{i=1}^{T_{g}}\frac{1}{\tilde{\sigma}%
_{i}^{2}}}\right) ^{2}+\frac{\sum_{i=1}^{T_{g}}\frac{\tilde{y}_{ig}^{2}}{%
\tilde{\sigma}_{i}^{2}}}{\frac{1}{\tau ^{2}}+\sum_{i=1}^{T_{g}}\frac{1}{%
\tilde{\sigma}_{i}^{2}}}\right) \right) d\mu _{g} \\
L_{g} &=&\frac{1}{2\pi }\frac{1}{\sqrt{\tau ^{2}}}\prod_{i=1}^{T_{g}}\frac{1%
}{\sqrt{\tilde{\sigma}_{i}^{2}}}\int_{-\infty }^{\infty }\exp \left( -\frac{1%
}{2}\left( \frac{1}{\tau ^{2}}+\sum_{i=1}^{T_{g}}\frac{1}{\tilde{\sigma}%
_{i}^{2}}\right) \left( \left( \mu _{g}^{2}-\frac{\sum_{i=1}^{T_{g}}\frac{%
\tilde{y}_{ig}}{\tilde{\sigma}_{i}^{2}}}{\frac{1}{\tau ^{2}}%
+\sum_{i=1}^{T_{g}}\frac{1}{\tilde{\sigma}_{i}^{2}}}\right) ^{2}+\frac{%
\sum_{i=1}^{T_{g}}\frac{\tilde{y}_{ig}^{2}}{\tilde{\sigma}_{i}^{2}}}{\frac{1%
}{\tau ^{2}}+\sum_{i=1}^{T_{g}}\frac{1}{\tilde{\sigma}_{i}^{2}}}-\left( 
\frac{\sum_{i=1}^{T_{g}}\frac{\tilde{y}_{ig}}{\tilde{\sigma}_{i}^{2}}}{\frac{%
1}{\tau ^{2}}+\sum_{i=1}^{T_{g}}\frac{1}{\tilde{\sigma}_{i}^{2}}}\right)
^{2}\right) \right) d\mu _{g}
\end{eqnarray*}%
Pulling constants out of integrand and "building" a normal pdf:%
\[
L_{g}=\frac{1}{2\pi }\sqrt{\frac{2\pi }{\left( \frac{1}{\tau ^{2}}%
+\sum_{i=1}^{T_{g}}\frac{1}{\tilde{\sigma}_{i}^{2}}\right) }}\frac{1}{\sqrt{%
\tau ^{2}}}\prod_{i=1}^{T_{g}}\frac{1}{\sqrt{\tilde{\sigma}_{i}^{2}}}\exp
\left( -\frac{1}{2}\left( \frac{1}{\tau ^{2}}+\sum_{i=1}^{T_{g}}\frac{1}{%
\tilde{\sigma}_{i}^{2}}\right) \left( \frac{\sum_{i=1}^{T_{g}}\frac{\tilde{y}%
_{ig}^{2}}{\tilde{\sigma}_{i}^{2}}}{\frac{1}{\tau ^{2}}+\sum_{i=1}^{T_{g}}%
\frac{1}{\tilde{\sigma}_{i}^{2}}}-\left( \frac{\sum_{i=1}^{T_{g}}\frac{%
\tilde{y}_{ig}}{\tilde{\sigma}_{i}^{2}}}{\frac{1}{\tau ^{2}}%
+\sum_{i=1}^{T_{g}}\frac{1}{\tilde{\sigma}_{i}^{2}}}\right) ^{2}\right)
\right) \int_{-\infty }^{\infty }\frac{1}{\sqrt{\frac{2\pi }{\left( \frac{1}{%
\tau ^{2}}+\sum_{i=1}^{T_{g}}\frac{1}{\tilde{\sigma}_{i}^{2}}\right) }}}\exp
\left( -\frac{1}{2}\frac{\left( \mu _{g}^{2}-\frac{\sum_{i=1}^{T_{g}}\frac{%
\tilde{y}_{ig}}{\tilde{\sigma}_{i}^{2}}}{\frac{1}{\tau ^{2}}%
+\sum_{i=1}^{T_{g}}\frac{1}{\tilde{\sigma}_{i}^{2}}}\right) ^{2}}{\frac{1}{%
\frac{1}{\tau ^{2}}+\sum_{i=1}^{T_{g}}\frac{1}{\tilde{\sigma}_{i}^{2}}}}%
\right) d\mu _{g} 
\]%
All PDFs integrate to one:%
\[
L_{g}=\frac{1}{\sqrt{2\pi }}\sqrt{\frac{1}{\left( 1+\sum_{i=1}^{T_{g}}\frac{%
\tau ^{2}}{\tilde{\sigma}_{i}^{2}}\right) }}\prod_{i=1}^{T_{g}}\frac{1}{%
\sqrt{\tilde{\sigma}_{i}^{2}}}\exp \left( -\frac{1}{2}\left( \frac{1}{\tau
^{2}}+\sum_{i=1}^{T_{g}}\frac{1}{\tilde{\sigma}_{i}^{2}}\right) \left( \frac{%
\sum_{i=1}^{T_{g}}\frac{\tilde{y}_{ig}^{2}}{\tilde{\sigma}_{i}^{2}}}{\frac{1%
}{\tau ^{2}}+\sum_{i=1}^{T_{g}}\frac{1}{\tilde{\sigma}_{i}^{2}}}-\left( 
\frac{\sum_{i=1}^{T_{g}}\frac{\tilde{y}_{ig}}{\tilde{\sigma}_{i}^{2}}}{\frac{%
1}{\tau ^{2}}+\sum_{i=1}^{T_{g}}\frac{1}{\tilde{\sigma}_{i}^{2}}}\right)
^{2}\right) \right) 
\]%
Taking logs and dropping constants:%
\[
\ln L_{g}=-\frac{1}{2}\ln \left( 1+\sum_{i=1}^{T_{g}}\frac{\tau ^{2}}{\tilde{%
\sigma}_{i}^{2}}\right) -\frac{1}{2}\sum_{i=1}^{T_{g}}\ln \left( \tilde{%
\sigma}_{i}^{2}\right) -\frac{1}{2}\left( \frac{1}{\tau ^{2}}%
+\sum_{i=1}^{T_{g}}\frac{1}{\tilde{\sigma}_{i}^{2}}\right) \left( \frac{%
\sum_{i=1}^{T_{g}}\frac{\tilde{y}_{ig}^{2}}{\tilde{\sigma}_{i}^{2}}}{\frac{1%
}{\tau ^{2}}+\sum_{i=1}^{T_{g}}\frac{1}{\tilde{\sigma}_{i}^{2}}}-\left( 
\frac{\sum_{i=1}^{T_{g}}\frac{\tilde{y}_{ig}}{\tilde{\sigma}_{i}^{2}}}{\frac{%
1}{\tau ^{2}}+\sum_{i=1}^{T_{g}}\frac{1}{\tilde{\sigma}_{i}^{2}}}\right)
^{2}\right) 
\]%
Multiply through by $-2$:%
\[
-2\ln L_{g}=\ln \left( 1+\sum_{i=1}^{T_{g}}\frac{\tau ^{2}}{\tilde{\sigma}%
_{i}^{2}}\right) +\ln \tau ^{2}+\sum_{i=1}^{T_{g}}\ln \left( \tilde{\sigma}%
_{i}^{2}\right) +\left( \frac{1}{\tau ^{2}}+\sum_{i=1}^{T_{g}}\frac{1}{%
\tilde{\sigma}_{i}^{2}}\right) \left( \frac{\sum_{i=1}^{T_{g}}\frac{\tilde{y}%
_{ig}^{2}}{\tilde{\sigma}_{i}^{2}}}{\frac{1}{\tau ^{2}}+\sum_{i=1}^{T_{g}}%
\frac{1}{\tilde{\sigma}_{i}^{2}}}-\left( \frac{\sum_{i=1}^{T_{g}}\frac{%
\tilde{y}_{ig}}{\tilde{\sigma}_{i}^{2}}}{\frac{1}{\tau ^{2}}%
+\sum_{i=1}^{T_{g}}\frac{1}{\tilde{\sigma}_{i}^{2}}}\right) ^{2}\right) 
\]%
Simplifying:%
\[
-2\ln L_{g}=\ln \left( 1+\sum_{i=1}^{T_{g}}\frac{\tau ^{2}}{\tilde{\sigma}%
_{i}^{2}}\right) +\sum_{i=1}^{T_{g}}\ln \left( \tilde{\sigma}_{i}^{2}\right)
+\left( \sum_{i=1}^{T_{g}}\frac{\tilde{y}_{ig}^{2}}{\tilde{\sigma}_{i}^{2}}-%
\frac{1}{\frac{1}{\tau ^{2}}+\sum_{i=1}^{T_{g}}\frac{1}{\tilde{\sigma}%
_{i}^{2}}}\left( \sum_{i=1}^{T_{g}}\frac{\tilde{y}_{ig}}{\tilde{\sigma}%
_{i}^{2}}\right) ^{2}\right) 
\]%
\[
-2\ln L_{g}=\sum_{i=1}^{T_{g}}\ln \left( \tilde{\sigma}_{i}^{2}\right) +\ln
\left( 1+\tau ^{2}\sum_{i=1}^{T_{g}}\frac{1}{\tilde{\sigma}_{i}^{2}}\right)
+\sum_{i=1}^{T_{g}}\frac{\tilde{y}_{ig}^{2}}{\tilde{\sigma}_{i}^{2}}-\left( 
\frac{1}{\tau ^{2}}+\sum_{i=1}^{T_{g}}\frac{1}{\tilde{\sigma}_{i}^{2}}%
\right) ^{-1}\left( \sum_{i=1}^{T_{g}}\frac{\tilde{y}_{ig}}{\tilde{\sigma}%
_{i}^{2}}\right) ^{2} 
\]

Checking what happens when measurement error is zero:%
\begin{eqnarray*}
-2\ln L_{g} &=&\ln \left( 1+\sum_{i=1}^{T_{g}}\frac{\tau ^{2}}{\sigma ^{2}}%
\right) +\sum_{i=1}^{T_{g}}\ln \left( \sigma ^{2}\right) +\left(
\sum_{i=1}^{T_{g}}\frac{\tilde{y}_{ig}^{2}}{\sigma ^{2}}-\frac{1}{\frac{1}{%
\tau ^{2}}+\sum_{i=1}^{T_{g}}\frac{1}{\sigma ^{2}}}\left( \sum_{i=1}^{T_{g}}%
\frac{\tilde{y}_{ig}}{\sigma ^{2}}\right) ^{2}\right) \\
&=&\ln \left( 1+\frac{T_{g}\tau ^{2}}{\sigma ^{2}}\right) +T_{g}\ln \left(
\sigma ^{2}\right) +\frac{1}{\sigma ^{2}}\left( \sum_{i=1}^{T_{g}}\tilde{y}%
_{ig}^{2}-\frac{\tau ^{2}}{\sigma ^{2}+T_{g}\tau ^{2}}\left(
\sum_{i=1}^{T_{g}}\tilde{y}_{ig}\right) ^{2}\right)
\end{eqnarray*}

\section{Derivation of Derivatives}

recall:%
\[
-2\ln L_{g}=\sum_{i=1}^{T_{g}}\ln \left( \tilde{\sigma}_{i}^{2}\right) +\ln
\left( 1+\tau ^{2}\sum_{i=1}^{T_{g}}\frac{1}{\tilde{\sigma}_{i}^{2}}\right)
+\sum_{i=1}^{T_{g}}\frac{\tilde{y}_{ig}^{2}}{\tilde{\sigma}_{i}^{2}}-\left( 
\frac{1}{\tau ^{2}}+\sum_{i=1}^{T_{g}}\frac{1}{\tilde{\sigma}_{i}^{2}}%
\right) ^{-1}\left( \sum_{i=1}^{T_{g}}\frac{\tilde{y}_{ig}}{\tilde{\sigma}%
_{i}^{2}}\right) ^{2} 
\]

\[
\tilde{y}_{ig}=y_{ig}-X_{i}\beta -\gamma \left( \frac{1}{T_{g}}%
\sum_{i=1}^{T_{g}}X_{i}\beta \right) 
\]%
\[
\frac{\partial \tilde{y}_{ig}}{\partial \left( X_{i}\beta \right) }=-\left(
1+\frac{\gamma }{T_{g}}\right) 
\]%
\[
\tilde{\sigma}_{i}^{2}=\sigma ^{2}+\eta _{i}^{2}. 
\]

derive:

\begin{eqnarray*}
\frac{\partial \left( -2\ln L_{g}\right) }{\partial \beta }
&=&\sum_{i=1}^{T_{g}}\frac{\partial \left( -2\ln L_{g}\right) }{\partial
\left( X_{i}\beta \right) }X_{i} \\
\frac{\partial \left( -2\ln L_{g}\right) }{\partial \left( X_{i}\beta
\right) } &=&\frac{\partial \tilde{y}_{ig}}{\partial \left( X_{i}\beta
\right) }\left( \frac{2\tilde{y}_{ig}}{\tilde{\sigma}_{i}^{2}}-\left( \frac{1%
}{\tau ^{2}}+\sum_{i=1}^{T_{g}}\frac{1}{\tilde{\sigma}_{i}^{2}}\right)
^{-1}2\left( \sum_{i=1}^{T_{g}}\frac{\tilde{y}_{ig}}{\tilde{\sigma}_{i}^{2}}%
\right) \left( \frac{1}{\tilde{\sigma}_{i}^{2}}\right) \right) \\
&=&2\frac{\partial \tilde{y}_{ig}}{\partial \left( X_{i}\beta \right) }%
\left( \frac{\tilde{y}_{ig}}{\tilde{\sigma}_{i}^{2}}-\left(
\sum_{i=1}^{T_{g}}\frac{\tilde{y}_{ig}}{\tilde{\sigma}_{i}^{2}}\right)
\left( \frac{1}{\tilde{\sigma}_{i}^{2}}\right) \left( \frac{1}{\tau ^{2}}%
+\sum_{i=1}^{T_{g}}\frac{1}{\tilde{\sigma}_{i}^{2}}\right) ^{-1}\right) \\
&=&-2\left( 1+\frac{\gamma }{T_{g}}\right) \left( \frac{\tilde{y}_{ig}}{%
\tilde{\sigma}_{i}^{2}}-\left( \sum_{i=1}^{T_{g}}\frac{\tilde{y}_{ig}}{%
\tilde{\sigma}_{i}^{2}}\right) \left( \frac{1}{\tilde{\sigma}_{i}^{2}}%
\right) \left( \frac{1}{\tau ^{2}}+\sum_{i=1}^{T_{g}}\frac{1}{\tilde{\sigma}%
_{i}^{2}}\right) ^{-1}\right)
\end{eqnarray*}

\bigskip

\[
-2\ln L_{g}=\sum_{i=1}^{T_{g}}\ln \left( \tilde{\sigma}_{i}^{2}\right) +\ln
\left( 1+\tau ^{2}\sum_{i=1}^{T_{g}}\frac{1}{\tilde{\sigma}_{i}^{2}}\right)
+\sum_{i=1}^{T_{g}}\frac{\tilde{y}_{ig}^{2}}{\tilde{\sigma}_{i}^{2}}-\left( 
\frac{1}{\tau ^{2}}+\sum_{i=1}^{T_{g}}\frac{1}{\tilde{\sigma}_{i}^{2}}%
\right) ^{-1}\left( \sum_{i=1}^{T_{g}}\frac{\tilde{y}_{ig}}{\tilde{\sigma}%
_{i}^{2}}\right) ^{2} 
\]%
\begin{eqnarray*}
\frac{\partial \left( -2\ln L_{g}\right) }{\partial \sigma }
&=&\sum_{i=1}^{T_{g}}\frac{\partial \left( -2\ln L_{g}\right) }{\tilde{\sigma%
}_{i}^{2}}\frac{\partial \tilde{\sigma}_{i}^{2}}{\partial \sigma } \\
&=&2\sigma \sum_{i=1}^{T_{g}}\frac{\partial \left( -2\ln L_{g}\right) }{%
\tilde{\sigma}_{i}^{2}} \\
&=&2\sigma \left[ \sum_{i=1}^{T_{g}}\frac{1}{\tilde{\sigma}_{i}^{2}}+\frac{%
\tau ^{2}\left( \sum_{i=1}^{T_{g}}\frac{-1}{\tilde{\sigma}_{i}^{4}}\right) }{%
1+\tau ^{2}\left( \sum_{i=1}^{T_{g}}\frac{1}{\tilde{\sigma}_{i}^{2}}\right) }%
+\sum_{i=1}^{T_{g}}-\frac{\tilde{y}_{ig}^{2}}{\tilde{\sigma}_{i}^{4}}-\left( 
\frac{1}{\tau ^{2}}+\sum_{i=1}^{T_{g}}\frac{1}{\tilde{\sigma}_{i}^{2}}%
\right) ^{-1}2\left( \sum_{i=1}^{T_{g}}\frac{\tilde{y}_{ig}}{\tilde{\sigma}%
_{i}^{2}}\right) \left( \sum_{i=1}^{T_{g}}\frac{-\tilde{y}_{ig}}{\tilde{%
\sigma}_{i}^{4}}\right) -\left( -1\right) \left( \frac{1}{\tau ^{2}}%
+\sum_{i=1}^{T_{g}}\frac{1}{\tilde{\sigma}_{i}^{2}}\right) ^{-2}\left(
\sum_{i=1}^{T_{g}}\frac{-1}{\tilde{\sigma}_{i}^{4}}\right) \left(
\sum_{i=1}^{T_{g}}\frac{\tilde{y}_{ig}}{\tilde{\sigma}_{i}^{2}}\right) ^{2}%
\right] \\
&=&2\sigma \left[ \sum_{i=1}^{T_{g}}\frac{1}{\tilde{\sigma}_{i}^{2}}-\frac{%
\tau ^{2}\left( \sum_{i=1}^{T_{g}}\frac{1}{\tilde{\sigma}_{i}^{4}}\right) }{%
1+\tau ^{2}\left( \sum_{i=1}^{T_{g}}\frac{1}{\tilde{\sigma}_{i}^{2}}\right) }%
-\sum_{i=1}^{T_{g}}\frac{\tilde{y}_{ig}^{2}}{\tilde{\sigma}_{i}^{4}}+2\left(
\sum_{i=1}^{T_{g}}\frac{\tilde{y}_{ig}}{\tilde{\sigma}_{i}^{2}}\right)
\left( \sum_{i=1}^{T_{g}}\frac{\tilde{y}_{ig}}{\tilde{\sigma}_{i}^{4}}%
\right) \left( \frac{1}{\tau ^{2}}+\sum_{i=1}^{T_{g}}\frac{1}{\tilde{\sigma}%
_{i}^{2}}\right) ^{-1}-\left( \sum_{i=1}^{T_{g}}\frac{\tilde{y}_{ig}}{\tilde{%
\sigma}_{i}^{2}}\right) ^{2}\left( \sum_{i=1}^{T_{g}}\frac{1}{\tilde{\sigma}%
_{i}^{4}}\right) \left( \frac{1}{\tau ^{2}}+\sum_{i=1}^{T_{g}}\frac{1}{%
\tilde{\sigma}_{i}^{2}}\right) ^{-2}\right]
\end{eqnarray*}%
\[
\frac{\partial \left( -2\ln L_{g}\right) }{\partial \tau }=2\tau \frac{%
\sum_{i=1}^{T_{g}}\frac{1}{\tilde{\sigma}_{i}^{2}}}{\left( 1+\tau
^{2}\sum_{i=1}^{T_{g}}\frac{1}{\tilde{\sigma}_{i}^{2}}\right) }-\frac{2}{%
\tau ^{3}}\left( \frac{1}{\tau ^{2}}+\sum_{i=1}^{T_{g}}\frac{1}{\tilde{\sigma%
}_{i}^{2}}\right) ^{-2}\left( \sum_{i=1}^{T_{g}}\frac{\tilde{y}_{ig}}{\tilde{%
\sigma}_{i}^{2}}\right) ^{2} 
\]

\begin{eqnarray*}
\frac{\partial \left( -2\ln L_{g}\right) }{\partial \gamma } &=&\left(
\sum_{i=1}^{T_{g}}\frac{2\tilde{y}_{ig}\left( -\left( \bar{X}_{g}\beta
\right) \right) }{\tilde{\sigma}_{i}^{2}}-\left( \frac{1}{\tau ^{2}}%
+\sum_{i=1}^{T_{g}}\frac{1}{\tilde{\sigma}_{i}^{2}}\right) ^{-1}2\left(
\sum_{i=1}^{T_{g}}\frac{\tilde{y}_{ig}}{\tilde{\sigma}_{i}^{2}}\right)
\sum_{i=1}^{T_{g}}\frac{-\bar{X}_{g}\beta }{\tilde{\sigma}_{i}^{2}}\right) \\
&=&-2\sum_{i=1}^{T_{g}}\frac{\tilde{y}_{ig}\left( \bar{X}_{g}\beta \right) }{%
\tilde{\sigma}_{i}^{2}}+2\left( \frac{1}{\tau ^{2}}+\sum_{i=1}^{T_{g}}\frac{1%
}{\tilde{\sigma}_{i}^{2}}\right) ^{-1}\left( \sum_{i=1}^{T_{g}}\frac{\tilde{y%
}_{ig}}{\tilde{\sigma}_{i}^{2}}\right) \sum_{i=1}^{T_{g}}\frac{\bar{X}%
_{g}\beta }{\tilde{\sigma}_{i}^{2}}
\end{eqnarray*}

\end{document}
